dev/lf/delayed-types/Precise_flow.v
@@ -117,6 +117,15 @@ Proof.
     specialize (IHHpf T eq_refl); inversion IHHpf.
 Qed.
 
+Lemma precise_flow_nref_inv : forall x G T U,
+    precise_flow x G (typ_nref T) U ->
+    U = (typ_nref T).
+Proof.
+  introv Hpf.
+  dependent induction Hpf; auto;
+    specialize (IHHpf T eq_refl); inversion IHHpf.
+Qed.
+
 Lemma precise_flow_bnd_eq_or_record : forall x G T,
     record_type T ->
     (forall U, precise_flow x G (typ_bnd T) U ->
