dev/lf/tight-proof/Some_lemmas.v
@@ -103,27 +103,22 @@ Qed.
 (* ###################################################################### *)
 (** *** Lemmas to upcast to general typing *)
 
-Lemma precise_to_general: forall m1 m2 G t T,
-    ty_trm m1 m2 G t T ->
-    m1 = ty_precise ->
-    m2 = sub_general ->
-    ty_trm ty_general sub_general G t T.
+Lemma precise_to_general: forall G t T,
+    ty_trm_p G t T ->
+    ty_trm G t T.
 Proof.
   intros. induction H; intros; subst; eauto.
 Qed.
 
 Lemma tight_to_general:
-  (forall m1 m2 G t T,
-     ty_trm m1 m2 G t T ->
-     m1 = ty_general ->
-     m2 = sub_tight ->
-     ty_trm ty_general sub_general G t T) /\
-  (forall m2 G S U,
-     subtyp m2 G S U ->
-     m2 = sub_tight ->
-     subtyp sub_general G S U).
+  (forall G t T,
+     ty_trm_t G t T ->
+     ty_trm G t T) /\
+  (forall G S U,
+     subtyp_t G S U ->
+     subtyp G S U).
 Proof.
-  apply ts_mutind; intros; subst; eauto.
+  apply ts_mutind_t; intros; subst; eauto.
   - apply precise_to_general in t; eauto.
   - apply precise_to_general in t; eauto.
 Qed.
@@ -132,7 +127,7 @@ Qed.
 (** *** Misc Lemmas *)
 
 Lemma var_typing_implies_avar_f: forall G a T,
-  ty_trm ty_general sub_general G (trm_var a) T ->
+  ty_trm G (trm_var a) T ->
   exists x, a = avar_f x.
 Proof.
   intros. dependent induction H; try solve [eexists; reflexivity].
@@ -140,21 +135,21 @@ Proof.
 Qed.
 
 Lemma val_typing: forall G v T,
-  ty_trm ty_general sub_general G (trm_val v) T ->
-  exists T', ty_trm ty_precise sub_general G (trm_val v) T' /\
-             subtyp sub_general G T' T.
+  ty_trm G (trm_val v) T ->
+  exists T', ty_trm_p G (trm_val v) T' /\
+             subtyp G T' T.
 Proof.
   intros G v T H. dependent induction H.
   - exists (typ_all T U). split.
-    apply ty_all_intro with (L:=L); eauto. apply subtyp_refl.
+    apply ty_all_intro_p with (L:=L); eauto. apply subtyp_refl.
   - exists (typ_bnd T). split.
-    apply ty_new_intro with (L:=L); eauto. apply subtyp_refl.
-  - destruct (IHty_trm _ eq_refl eq_refl eq_refl) as [T' [Hty Hsub]].
+    apply ty_new_intro_p with (L:=L); eauto. apply subtyp_refl.
+  - destruct (IHty_trm _ eq_refl) as [T' [Hty Hsub]].
     exists T'. split; eauto.
 Qed.
 
-Lemma typing_implies_bound: forall m1 m2 G x T,
-  ty_trm m1 m2 G (trm_var (avar_f x)) T ->
+Lemma typing_implies_bound: forall G x T,
+  ty_trm G (trm_var (avar_f x)) T ->
   exists S, binds x S G.
 Proof.
   intros. remember (trm_var (avar_f x)) as t.
@@ -163,4 +158,13 @@ Proof.
     try solve [inversion Heqt; eapply IHty_trm; eauto];
     try solve [inversion Heqt; eapply IHty_trm1; eauto].
   - inversion Heqt. subst. exists T. assumption.
+Qed.
+
+Lemma precise_typing_implies_bound: forall G x T,
+  ty_trm_p G (trm_var (avar_f x)) T ->
+  exists S, binds x S G.
+Proof.
+  intros. 
+  pose proof (precise_to_general H) as H'.
+  pose proof (typing_implies_bound H'). assumption.
 Qed.
