dev/lf/tight-proof/Wellformed_store.v
@@ -21,7 +21,7 @@ Hint Resolve wf_sto_to_ok_G.
 
 Lemma tpt_to_precise_rec: forall G v T,
     tight_pt_v G v (typ_bnd T) ->
-    ty_trm ty_precise sub_general G (trm_val v) (typ_bnd T).
+    ty_trm_p G (trm_val v) (typ_bnd T).
 Proof.
   introv Ht.
   inversions Ht. assumption.
@@ -31,10 +31,10 @@ Lemma tpt_to_precise_lambda: forall G v S T,
     tight_pt_v G v (typ_all S T) ->
     inert G ->
     exists L S' T',
-      ty_trm ty_precise sub_general G (trm_val v) (typ_all S' T') /\
-      subtyp sub_general G S S' /\
+      ty_trm_p G (trm_val v) (typ_all S' T') /\
+      subtyp G S S' /\
       (forall y, y \notin L ->
-                 subtyp sub_general (G & y ~ S) (open_typ y T') (open_typ y T)).
+                 subtyp (G & y ~ S) (open_typ y T') (open_typ y T)).
 Proof.
   introv Ht Hg. dependent induction Ht.
   - exists (dom G) S T. split*.
@@ -51,7 +51,7 @@ Proof.
 Qed.
 
 Lemma precise_forall_inv : forall G v S T,
-    ty_trm ty_precise sub_general G (trm_val v) (typ_all S T) ->
+    ty_trm_p G (trm_val v) (typ_all S T) ->
     exists t,
       v = val_lambda S t.
 Proof.
@@ -59,7 +59,7 @@ Proof.
 Qed.
 
 Lemma precise_bnd_inv : forall G v S,
-    ty_trm ty_precise sub_general G (trm_val v) (typ_bnd S) ->
+    ty_trm_p G (trm_val v) (typ_bnd S) ->
     exists ds,
       v = val_new S ds.
 Proof.
@@ -67,7 +67,7 @@ Proof.
 Qed.
 
 Lemma precise_obj_typ : forall G T ds U,
-    ty_trm ty_precise sub_general G (trm_val (val_new T ds)) U ->
+    ty_trm_p G (trm_val (val_new T ds)) U ->
     U = typ_bnd T.
 Proof.
   introv Hp. dependent induction Hp; auto.
@@ -87,13 +87,13 @@ Lemma corresponding_types: forall G s x T,
   inert G ->
   binds x T G ->
   ((exists L S U S' U' t, binds x (val_lambda S t) s /\
-                  ty_trm ty_precise sub_general G (trm_val (val_lambda S t)) (typ_all S U) /\
+                  ty_trm_p G (trm_val (val_lambda S t)) (typ_all S U) /\
                   T = typ_all S' U' /\
-                  subtyp sub_general G S' S /\
+                  subtyp G S' S /\
                   (forall y, y \notin L ->
-                  subtyp sub_general (G & y ~ S') (open_typ y U) (open_typ y U'))) \/
+                  subtyp (G & y ~ S') (open_typ y U) (open_typ y U'))) \/
    (exists S ds, binds x (val_new S ds) s /\
-                 ty_trm ty_precise sub_general G (trm_val (val_new S ds)) (typ_bnd S) /\
+                 ty_trm_p G (trm_val (val_new S ds)) (typ_bnd S) /\
                  T = typ_bnd S)).
 Proof.
   introv H Hgd Bi. induction H.
